refactor: make `Ctxt` a newtype structure instead of a def (#1452)
This PR changes the `Ctxt Ty` type to be a structure with a single field
of type `List Ty` instead of a `def` defined as the same. This way, the
conversion from Ctxt to List becomes an explicit `toList / ofList`
definition in the expression, which we can then match on in simp
rewrites.
More importantly, it ensures we can add instances on Ctxt which might
behave differently from the corresponding List instance, without
inviting dependent-typed hell. For example, we might want to define what
it means to append a list of types to a context, and we might want the
order of the result to be slightly different from what appending the
underlying lists would give us.

I'm not quite sure why, but this change triggered some bugs related to
termination checking in some of the trickier mutually recursive
functions (e.g., `matchVar`/`matchArg`). I added explicit termination_by
hints to guide the checker, but this changed the error from a failure to
check termination into:
```
Cannot derive matchArg._mutual.eq_def
  failed to generate splitter for match auxiliary declaration 'matchVar.match_3', unsolved subgoal:
```
I eventually figured that moving the match on the variable `w : Var
Δ_out t` from the top-level matcharms down into a separate match just on
`w` avoids the error. Why? Who knows?

This error seems to have been the root-cause of the termination checker
failure: after this match-change we can remove the explicit termination
hints and the termination checker will find the right bounds
automatically again. However, it seemed more robust to me to leave them
in, in case we run into similar issues in the future.

SSA/Core/ErasedContext.lean
@@ -19,84 +19,101 @@ notation "⟦" x "⟧" => TyDenote.toType x
 
 instance : TyDenote Unit where toType := fun _ => Unit
 
-def Ctxt (Ty : Type) : Type :=
+structure Ctxt (Ty : Type) : Type where
+  ofList :: toList : List Ty
   -- Erased <| List Ty
-  List Ty
+  deriving Repr, Lean.ToExpr
 
-abbrev Ctxt.toList (Γ : Ctxt Ty) : List Ty := Γ
+attribute [coe] Ctxt.ofList
 
 namespace Ctxt
 
 variable {Ty : Type}
 
-/-! ### Inherited Instances-/
-/-- `inherit_instance Foo` wil define an instance of `[Foo Ty] → Foo (Ctxt Ty)`,
-  assuming an instance of `Foo` exists for `List` -/
-local macro "inherit_instance" cls:term : command =>
-  `(instance {Ty : Type} [$cls Ty] : $cls (Ctxt Ty) := inferInstanceAs <| $cls (List Ty))
-inherit_instance Repr
-inherit_instance Lean.ToMessageData
+/-! ### Typeclass Instances-/
+section Instances
 
--- def empty : Ctxt := Erased.mk []
-def empty : Ctxt Ty := []
+open Lean in
+instance [ToMessageData Ty] : ToMessageData (Ctxt Ty) where
+  toMessageData (Γ) := m!"{Γ.toList}"
+
+instance : Coe (List Ty) (Ctxt Ty) where
+  coe := ofList
+
+end Instances
+
+def empty : Ctxt Ty := .ofList []
 
 instance : EmptyCollection (Ctxt Ty) := ⟨Ctxt.empty⟩
 instance : Inhabited (Ctxt Ty) := ⟨Ctxt.empty⟩
 
-lemma empty_eq : (∅ : Ctxt Ty) = [] := rfl
+lemma empty_eq : (∅ : Ctxt Ty) = .empty := rfl
 
 @[match_pattern]
-def snoc : Ctxt Ty → Ty → Ctxt Ty :=
-  -- fun tl hd => do return hd :: (← tl)
-  fun tl hd => hd :: tl
+def snoc : Ctxt Ty → Ty → Ctxt Ty
+  | ⟨tl⟩, hd => ⟨hd :: tl⟩
 
-/-- Turn a list of types into a context -/
-@[coe, simp]
-def ofList : List Ty → Ctxt Ty :=
-  -- Erased.mk
-  fun Γ => Γ
+instance : GetElem? (Ctxt Ty) Nat Ty (fun as i => i < as.toList.length) where
+  getElem xs i h := xs.toList[i]
+  getElem? xs i  := xs.toList[i]?
 
-
-instance : GetElem (Ctxt Ty) Nat Ty (fun as i => i < as.length) :=
-  inferInstanceAs (GetElem (List _) ..)
-instance : GetElem? (Ctxt Ty) Nat Ty (fun as i => i < as.length) :=
-  inferInstanceAs (GetElem? (List _) ..)
-
--- Why was this noncomutable? (removed it to make transformation computable)
-@[simp]
-def get? : Ctxt Ty → Nat → Option Ty :=
-  GetElem?.getElem? (coll := List _)
+@[simp
+-- , deprecated "Use `getElem?`" (since := "")
+]
+def get? : Ctxt Ty → Nat → Option Ty := (·[·]?)
 
 /-- Map a function from one type universe to another over a context -/
 def map (f : Ty₁ → Ty₂) : Ctxt Ty₁ → Ctxt Ty₂ :=
-  List.map f
+  ofList ∘ (List.map f) ∘ toList
 
-@[simp]
-lemma map_nil (f : Ty → Ty') :
-  map f ∅ = ∅ := rfl
+def length (Γ : Ctxt Ty) : Nat := Γ.toList.length
 
-@[simp]
-lemma map_cons (Γ : Ctxt Ty) (t : Ty) (f : Ty → Ty') :
-  map f (Γ.cons t) = (Γ.map f).cons (f t) := rfl
+section Lemmas
+variable (Γ : Ctxt Ty) (ts : List Ty)
 
-theorem map_snoc (Γ : Ctxt Ty) : (Γ.snoc a).map f = (Γ.map f).snoc (f a) := rfl
+lemma getElem?_eq_toList_getElem? {i : Nat} : Γ[i]? = Γ.toList[i]? := rfl
+@[simp] lemma getElem?_ofList (i : Nat) : (ofList ts)[i]? = ts[i]? := rfl
+
+@[simp] lemma getElem?_snoc_zero (t : Ty)           : (Γ.snoc t)[0]? = some t := rfl
+@[simp] lemma getElem?_snoc_succ (t : Ty) (i : Nat) : (Γ.snoc t)[i+1]? = Γ[i]? := rfl
+
+@[simp] lemma map_nil (f : Ty → Ty') : map f ∅ = ∅ := rfl
+@[simp] lemma map_snoc : (Γ.snoc a).map f = (Γ.map f).snoc (f a) := rfl
+
+@[simp] lemma getElem?_map (Γ : Ctxt Ty) (f : Ty → Ty') (i : Nat) :
+    (Γ.map f)[i]? = Γ[i]?.map f := by
+  simp [map]; rfl
+
+@[simp] lemma length_ofList : (ofList ts).length = ts.length := rfl
+@[simp] lemma length_snoc (Γ : Ctxt α) (x : α) : (Γ.snoc x).length = Γ.length + 1 := rfl
+@[simp] lemma length_map : (Γ.map f).length = Γ.length := by simp [map, length]
 
 instance : Functor Ctxt where
   map := map
 
+@[simp] lemma map_eq_map : f <$> Γ = map f Γ := rfl
+
 instance : LawfulFunctor Ctxt where
-  comp_map  := by simp only [List.map_eq_map, List.map_map, forall_const, implies_true]
-  id_map    := by simp only [List.map_eq_map, List.map_id, forall_const]
+  comp_map  := by simp [(· <$> ·), map]
+  id_map    := by simp [(· <$> ·), map]
   map_const := by simp only [Functor.mapConst, Functor.map, forall_const]
+
+end Lemmas
+
+section Rec
 
 /-- Recursion principle for contexts in terms of `Ctxt.nil` and `Ctxt.snoc` -/
 @[elab_as_elim, induction_eliminator]
-def recOn {motive : Ctxt Ty → Sort*}
+def recOn' {motive : Ctxt Ty → Sort*}
     (nil  : motive empty)
     (snoc : (Γ : Ctxt Ty) → (t : Ty) → motive Γ → motive (Γ.snoc t)) :
     ∀ Γ, motive Γ
-  | []        => nil
-  | ty :: tys  => snoc tys ty (recOn nil snoc tys)
+  | ⟨[]⟩        => nil
+  | ⟨ty :: tys⟩ => snoc ⟨tys⟩ ty (recOn' nil snoc ⟨tys⟩)
+
+end Rec
+
+/-! ## Variables -/
 
 def Var (Γ : Ctxt Ty) (t : Ty) : Type :=
   { i : Nat // Γ.get? i = some t }
@@ -115,10 +132,9 @@ instance : DecidableEq (Var Γ t) := by
 def last (Γ : Ctxt Ty) (t : Ty) : Ctxt.Var (Ctxt.snoc Γ t) t :=
   ⟨0, by rfl⟩
 
-def emptyElim {α : Sort _} {t : Ty} : Ctxt.Var [] t → α :=
+def emptyElim {α : Sort _} {t : Ty} : Ctxt.Var ∅ t → α :=
   fun ⟨_, h⟩ => by
-    simp only [get?, List.getElem?_nil, reduceCtorEq] at h
-
+    simp [getElem?_eq_toList_getElem?, EmptyCollection.emptyCollection, empty] at h
 
 /-- Take a variable in a context `Γ` and get the corresponding variable
 in context `Γ.snoc t`. This is marked as a coercion. -/
@@ -138,11 +154,7 @@ theorem succ_eq_toSnoc {Γ : Ctxt Ty} {t : Ty} {w} (h : (Γ.snoc t).get? (w+1) =
 
 /-- Transport a variable from `Γ` to any mapped context `Γ.map f` -/
 def toMap : Var Γ t → Var (Γ.map f) (f t)
-  | ⟨i, h⟩ => ⟨i, by
-      simp only [get?, map, List.getElem?_map, Option.map_eq_some_iff]
-      simp only [get?] at h
-      simp [h]
-    ⟩
+  | ⟨i, h⟩ => ⟨i, by simp_all⟩
 
 def cast {Γ : Ctxt Op} (h_eq : ty₁ = ty₂) : Γ.Var ty₁ → Γ.Var ty₂
   | ⟨i, h⟩ => ⟨i, h_eq ▸ h⟩
@@ -177,9 +189,7 @@ def casesOn
   match v with
     | ⟨0, h⟩ =>
         _root_.cast (by
-          simp only [get?, snoc, List.length_cons, Nat.zero_lt_succ, List.getElem?_eq_getElem,
-            List.getElem_cons_zero, Option.some.injEq] at h
-          subst h
+          obtain rfl : t' = t := by simpa [snoc] using h
           simp_all only [get?, zero_eq_last]
           ) <| @last Γ t
     | ⟨i+1, h⟩ =>
@@ -209,8 +219,6 @@ def casesOn_toSnoc
       Ctxt.Var.casesOn (motive := motive) (Ctxt.Var.toSnoc (t' := t') v) base last = base v :=
   rfl
 
-end Var
-
 theorem toSnoc_injective {Γ : Ctxt Ty} {t t' : Ty} :
     Function.Injective (@Ctxt.Var.toSnoc Ty Γ t t') := by
   let ofSnoc : (Γ.snoc t').Var t → Option (Γ.Var t) :=
@@ -218,6 +226,27 @@ theorem toSnoc_injective {Γ : Ctxt Ty} {t t' : Ty} :
   intro x y h
   simpa (config := { zetaDelta := true }) only [Var.casesOn_toSnoc, Option.some.injEq] using
     congr_arg ofSnoc h
+
+
+/-! ### Var Fin Helpers -/
+variable {Γ : Ctxt Ty}
+
+def toFin : Γ.Var t → Fin Γ.length
+  | ⟨idx, h⟩ => ⟨idx, by
+      suffices ¬(Γ.length ≤ idx) by omega
+      rcases Γ
+      simp only [length_ofList, ← List.getElem?_eq_none_iff]
+      simp_all
+    ⟩
+
+def ofFin : (i : Fin Γ.length) → Γ.Var (Γ[i])
+  | ⟨idx, h⟩ => ⟨idx, by simpa using List.getElem?_eq_getElem _⟩
+
+end Var
+
+/-!
+## Context Homomorphisms
+-/
 
 abbrev Hom (Γ Γ' : Ctxt Ty) := ⦃t : Ty⦄ → Γ.Var t → Γ'.Var t
 
@@ -283,9 +312,9 @@ def Valuation.eval {Γ : Ctxt Ty} (VAL : Valuation Γ) ⦃t : Ty⦄ (v : Γ.Var 
     VAL v
 
 /-- Make a valuation for the empty context. -/
-def Valuation.nil : Ctxt.Valuation ([] : Ctxt Ty) := fun _ v => v.emptyElim
+def Valuation.nil : Ctxt.Valuation (∅ : Ctxt Ty) := fun _ v => v.emptyElim
 
-instance : Inhabited (Ctxt.Valuation ([] : Ctxt Ty)) := ⟨Valuation.nil⟩
+instance : Inhabited (Ctxt.Valuation (∅ : Ctxt Ty)) := ⟨Valuation.nil⟩
 
 /-- Make a valuation for `Γ.snoc t` from a valuation for `Γ` and an element of `t.toType`. -/
 def Valuation.snoc {Γ : Ctxt Ty} {t : Ty} (s : Γ.Valuation) (x : toType t) :
@@ -302,8 +331,8 @@ infixl:50 "::ᵥ" => Valuation.snoc
 theorem Valuation.snoc_eq {Γ : Ctxt Ty} {t : Ty} (s : Γ.Valuation) (x : toType t) :
     (s.snoc x) = fun t var => match var with
       | ⟨0, hvar⟩ => by
-          simp only [get?, Ctxt.snoc, List.getElem?_cons_zero, Option.some.injEq] at hvar
-          exact (hvar ▸ x)
+          obtain rfl : _ = t := by simpa using hvar
+          exact x
       | ⟨.succ i, hvar⟩ => s ⟨i, hvar⟩ := by
   funext t' v
   rcases v with ⟨⟨⟩|i, hi⟩
@@ -335,8 +364,7 @@ theorem Valuation.snoc_toSnoc {Γ : Ctxt Ty} {t t' : Ty} (s : Γ.Valuation) (x :
 @[simp]
 theorem Valuation.snoc_eval {ty : Ty} (Γ : Ctxt Ty) (V : Γ.Valuation) (v : ⟦ty⟧)
     (hvar : Ctxt.get? (Ctxt.snoc Γ ty) (n+1) = some var_val) :
-    (V.snoc v) ⟨n+1, hvar⟩ = V ⟨n, by
-      simp only [get?, Ctxt.snoc, List.getElem?_cons_succ] at hvar; exact hvar⟩ :=
+    (V.snoc v) ⟨n+1, hvar⟩ = V ⟨n, by simpa using hvar⟩ :=
   rfl
 
 /-- There is only one distinct valuation for the empty context -/
@@ -350,13 +378,13 @@ theorem Valuation.snoc_toSnoc_last {Γ : Ctxt Ty} {t : Ty} (V : Valuation (Γ.sn
   cases v using Var.casesOn <;> rfl
 
 /-- Make a a valuation for a singleton value -/
-def Valuation.singleton {t : Ty} (v : toType t) : Ctxt.Valuation [t] :=
+def Valuation.singleton {t : Ty} (v : toType t) : Ctxt.Valuation ⟨[t]⟩ :=
   Ctxt.Valuation.nil.snoc v
 
 /-- Build valuation from a vector of values of types `types`. -/
 def Valuation.ofHVector {types : List Ty} : HVector toType types → Valuation (Ctxt.ofList types)
-  | .nil => (default : Ctxt.Valuation ([] : Ctxt Ty))
-  | .cons x xs => (Valuation.ofHVector xs).snoc x
+  | .nil        => (default : Ctxt.Valuation ∅)
+  | .cons x xs  => (Valuation.ofHVector xs).snoc x
 
 /-- Build valuation from a vector of values of types `types`. -/
 def Valuation.ofPair  {t₁ t₂ : Ty} (v₁: ⟦t₁⟧) (v₂ : ⟦t₂⟧) :
@@ -433,7 +461,7 @@ theorem Valuation.reassignVar_eq_of_lookup [DecidableEq Ty]
   rfl
 
 /-- Show that a valuation is equivalent to a `HVector` -/
-def Valuation.equivHVector {Γ : Ctxt Ty} : Valuation Γ ≃ HVector toType Γ where
+def Valuation.equivHVector {Γ : List Ty} : Valuation ⟨Γ⟩ ≃ HVector toType Γ where
   toFun V   := HVector.ofFn _ _ <| fun i => V ⟨i, by simp⟩
   invFun    := Valuation.ofHVector
   left_inv V := by
@@ -443,7 +471,7 @@ def Valuation.equivHVector {Γ : Ctxt Ty} : Valuation Γ ≃ HVector toType Γ w
     case nil =>
       rcases v with ⟨_, _⟩
       contradiction
-    case snoc Γ u ih =>
+    case cons Γ u ih =>
       cases v
       case last   => rfl
       case toSnoc => apply ih (fun t v => V v.toSnoc)
@@ -482,7 +510,7 @@ theorem val_toSnoc {Γ : Ctxt Ty} {t t' : Ty} (v : Γ.Var t) : (@toSnoc _ _ _ t'
   rfl
 
 instance : Repr (Var Γ t) where
-  reprPrec v _ := f!"%{Γ.length - v.val - 1}"
+  reprPrec v _ := f!"%{Γ.toList.length - v.val - 1}"
 
 end Var
 
@@ -535,8 +563,8 @@ def unSnoc (d : Diff (Γ₁.snoc t) Γ₂) : Diff Γ₁ Γ₂ :=
 def toMap (d : Diff Γ₁ Γ₂) : Diff (Γ₁.map f) (Γ₂.map f) :=
   ⟨d.val, by
     rcases d with ⟨d, h_get_d⟩
-    simp only [Valid, get?, map, List.getElem?_map, Option.map_eq_some_iff,
-      forall_exists_index, and_imp, forall_apply_eq_imp_iff₂] at h_get_d ⊢
+    simp only [Valid, get?, getElem?_map, Option.map_eq_some_iff, forall_exists_index, and_imp,
+      forall_apply_eq_imp_iff₂] at h_get_d ⊢
     intros a b c
     simp [h_get_d c]
   ⟩
@@ -568,6 +596,7 @@ theorem Valid.of_succ {Γ₁ Γ₂ : Ctxt Ty} {d : Nat} (h_valid : Valid Γ₁ (
     Valid Γ₁ Γ₂ d := by
   intro i t h_get
   simp [←h_valid h_get, snoc, List.getElem?_cons]
+  rfl
 
 lemma toHom_succ {Γ₁ Γ₂ : Ctxt Ty} {d : Nat} (h : Valid Γ₁ (Γ₂.snoc t) (d+1)) :
     toHom ⟨d+1, h⟩ = (toHom ⟨d, Valid.of_succ h⟩).snocRight := by
@@ -620,12 +649,12 @@ abbrev ofCtxt (Γ : Ctxt Ty) : DerivedCtxt Γ := ⟨Γ, .zero _⟩
 /-- value of a dervied context from an empty context,
      is the empty context with a zero diff. -/
 @[simp]
-theorem ofCtxt_empty : DerivedCtxt.ofCtxt ([] : Ctxt Ty) = ⟨[], .zero _⟩ := rfl
+theorem ofCtxt_empty : DerivedCtxt.ofCtxt (∅ : Ctxt Ty) = ⟨∅, .zero _⟩ := rfl
 
 /-- `snoc` of a derived context applies `snoc` to the underlying context, and updates the diff -/
 @[simp]
 def snoc {Γ : Ctxt Ty} : DerivedCtxt Γ → Ty → DerivedCtxt Γ
-  | ⟨ctxt, diff⟩, ty => ⟨ty::ctxt, diff.toSnoc⟩
+  | ⟨⟨Δ⟩, diff⟩, ty => ⟨ty::Δ, diff.toSnoc⟩
 
 theorem snoc_ctxt_eq_ctxt_snoc:
     (DerivedCtxt.snoc Γ ty).ctxt = Ctxt.snoc Γ.ctxt ty := by
@@ -651,7 +680,7 @@ end DerivedCtxt
 
 /-- `Γ.dropUntil v` is the largest prefix of context `Γ` that no longer contains variable `v` -/
 def dropUntil (Γ : Ctxt Ty) (v : Var Γ ty) : Ctxt Ty :=
-  List.drop (v.val + 1) Γ
+  ⟨List.drop (v.val + 1) Γ.toList⟩
 
 @[simp] lemma dropUntil_last   : dropUntil (snoc Γ ty) (Var.last Γ ty) = Γ := rfl
 @[simp] lemma dropUntil_toSnoc : dropUntil (snoc Γ ty) (Var.toSnoc v) = dropUntil Γ v := rfl
@@ -686,9 +715,6 @@ instance : CoeOut (Var (Γ.dropUntil v) ty) (Var Γ ty) where
 section ToExpr
 open Lean Qq
 variable [ToExpr Ty] {Γ : Ctxt Ty} {ty : Ty}
-
-instance : ToExpr (Ctxt Ty) :=
-  inferInstanceAs <| ToExpr (List Ty)
 
 /-- Construct an expression of type `Var Γ ty`.
 
@@ -733,7 +759,8 @@ def Valuation.mkOfElems (Ty instTyDenote : Expr) (Γ : Array Expr) (xs : Array E
     let mut V_acc := mkApp2 (mkConst ``Ctxt.Valuation.nil) Ty instTyDenote
     let mut Γ_acc := mkApp (.const ``List.nil [0]) Ty
     for (ty, x) in Γ.zip xs do
-      V_acc := mkApp6 (mkConst ``Ctxt.Valuation.snoc) Ty instTyDenote Γ_acc ty V_acc x
+      let Γ := mkApp2 (mkConst ``Ctxt.ofList) Ty Γ_acc
+      V_acc := mkApp6 (mkConst ``Ctxt.Valuation.snoc) Ty instTyDenote Γ ty V_acc x
       Γ_acc := mkApp3 (.const ``List.cons [0]) Ty ty Γ_acc
     V_acc
 
